Simulator/Lib.hs
@@ -39,7 +39,7 @@ getArgVal name n = do
 -- printVal :: T.FullFormat -> Val -> IO String
 -- printVal (T.FBool n bf) (BoolVal b) = return $ space_pad n (if b then "1" else "0")
 -- printVal (T.FBit n m bf) (BVVal bs) = return $ space_pad m $ printNum bf bs
--- printVal (T.FStruct n _ names ffs) (StructVal fields) = do
+-- printVal (T.FStruct n kindNames ffs) (StructVal fields) = do
 --     ps <- pair_sequence $ zipWith (\(name,val) ff -> (name, printVal ff val)) fields (map ffs $ T.getFins n)
 --     return ("{ " ++ concatMap (\(name,pval) -> name ++ ":" ++ pval ++ "; ") ps ++ "}")
 -- printVal (T.FArray n k ff) (ArrayVal vals) = do
